share1OneFracMinimal.bpl
@@ -1,70 +1,68 @@
 type Ref;
-type PredicateTypes;
-type FractionType = [Ref, PredicateTypes] int;
-type PackedType = [Ref, PredicateTypes] bool;
+type FractionType = [Ref] int;
+type PackedType = [Ref] bool;
 var packed: PackedType;
 var frac: FractionType;
 const null: Ref;
 
-var dc: [Ref]Ref;
+var packedShareCount: PackedType;
+var fracShareCount: FractionType;
 
-const unique ShareCountP: PredicateTypes;
+var dc: [Ref]Ref;
 
 procedure ConstructShare0(this:Ref, dc_:Ref);
 	ensures (dc[this] == dc_) &&
-		(packed[this, ShareCountP]) && 
-		(frac[this, ShareCountP] >= 100);
-
-procedure ConstructShare(this:Ref, dc_:Ref);
-	ensures (dc[this] == dc_);
+		(packedShareCount[this]) && 
+		(fracShareCount[this] >= 100);
 
 procedure PackShareCount(this:Ref);
-	requires (packed[dc[this], OKP] && 
-		(frac[dc[this], OKP] >= 1));
+	requires (packedOK[dc[this]] && 
+		(fracOK[dc[this]] >= 1));
 
 procedure UnpackShareCount(this:Ref);
-	requires packed[this, ShareCountP];
-	ensures (packed[dc[this], OKP] && 
-		(frac[dc[this], OKP] >= 1));
+	requires packedShareCount[this];
+	ensures (packedOK[dc[this]] && 
+		(fracOK[dc[this]] >= 1));
 
 procedure touch(this: Ref)
-	modifies val, dbl, packed;
-	requires packed[this, ShareCountP];
-	requires (frac[this, ShareCountP] >= 1);
-	ensures packed[this, ShareCountP] &&
-		(frac[this, ShareCountP] >= 1);
-
-	free ensures (forall x : Ref, y : PredicateTypes :: 
-		(
-		!((x==this) && (y==ShareCountP))
-		==> (packed[x,y]==old(packed[x,y]))
-		)
-	);
+	modifies val, dbl, packedShareCount, packedOK;
+	requires packedShareCount[this];
+	requires (fracShareCount[this] >= 1);
+	ensures packedShareCount[this] &&
+		(fracShareCount[this] >= 1);
+  ensures (forall x:Ref :: (packedOK[x] == old(packedOK[x])));
+  ensures (forall x:Ref :: (packedShareCount[x] == old(packedShareCount[x])));
 {
 	call UnpackShareCount(this);
-	packed[this, ShareCountP]:=false;
+	packedShareCount[this]:=false;
 	call increment(dc[this]) ;
 	call PackShareCount(this);
-	packed[this, ShareCountP]:=true;
+	packedShareCount[this]:=true;
 }
 
 procedure main()
-	modifies val, dbl, packed, frac;
+	modifies val, dbl, packedShareCount, packedOK, fracOK, fracShareCount;
 {
 	var dc0 : Ref;
 	var share1, share2 : Ref;
-	call ConstructDoubleCount0(dc0, 2, 4);
+	call ConstructDoubleCountOK(2, 4, dc0);
+
 	call ConstructShare0(share1, dc0);
+
 	call ConstructShare0(share2, dc0);
+
 	call PackShareCount(share1);
-	packed[share1, ShareCountP] := true;
-	frac[dc[share1], OKP] := frac[dc[share1], OKP] - 1;
+	packedShareCount[share1] := true;
+	fracOK[dc[share1]] := fracOK[dc[share1]] - 1;
+
 	call PackShareCount(share2);
-	packed[share2, ShareCountP] := true;
-	frac[dc[share2], OKP] := frac[dc[share2], OKP] - 1;
+	packedShareCount[share2] := true;
+	fracOK[dc[share2]] := fracOK[dc[share2]] - 1;
+
 	call touch(share1);
-	frac[share1, ShareCountP] := frac[share1, ShareCountP] -1;
+	fracShareCount[share1] := fracShareCount[share1] -1;
+
 	call touch(share2);
-	frac[share2, ShareCountP] := frac[share2, ShareCountP] -1;
+	fracShareCount[share2] := fracShareCount[share2] -1;
 }
 
